Source/PS.v
@@ -1,5 +1,3 @@
-Require Import Coq.Classes.Morphisms.
-
 Require Import Common.Definitions.
 Require Import Common.Util.
 Require Import Common.Values.
@@ -9,8 +7,6 @@ Require Import CompCert.Smallstep.
 Require Import Source.Language.
 Require Import Source.GlobalEnv.
 Require Import Source.CS.
-
-Require Import Coq.Setoids.Setoid.
 
 Module PS.
 
